src/program_proof/twophase/op_wrappers.v
@@ -16,12 +16,12 @@ From Goose Require github_com.mit_pdos.goose_nfsd.txn.
 From Goose Require github_com.mit_pdos.goose_nfsd.util.
 
 (* XXX: replace with the actual Goose generated version later *)
-Module TP.
+Module TwoPhasePre.
   Definition S := struct.decl [
     "txn" :: struct.ptrT txn.Txn.S;
     "locks" :: struct.ptrT lockmap.LockMap.S
   ].
-End TP.
+End TwoPhasePre.
 
 Definition TwoPhase__ReadBuf' : val :=
   λ: "twophase" "addr" "sz", SliceToList byteT (TwoPhase__ReadBuf "twophase" "addr" "sz").
@@ -31,7 +31,11 @@ Definition TwoPhase__OverWrite' : val :=
   let: "s" := ListToSlice byteT "data" in
   TwoPhase__OverWrite "twophase" "addr" "s" (slice.len "s").
 
-  (* XXX: todo: this should call a wrapped version of MkTxn that also allocates
-  the lockmap and returns a struct containing both *)
+(* XXX: todo: this should call a wrapped version of MkTxn that also allocates
+the lockmap and returns a struct containing both *)
 Definition TwoPhase__Init' : val :=
   (λ: "_", MkTxn #()).
+
+(* XXX: todo: this should be a version that takes a struct instead of the two arg version *)
+Definition TwoPhase__Begin' : val :=
+  (λ: "l", Begin "l").
