src/program_proof/twophase/wrapper_proof.v
@@ -1,0 +1,130 @@
+From Perennial.goose_lang Require Import lang notation typing.
+From Perennial.goose_lang.lib Require Import map.impl list.impl list_slice.
+From Perennial.goose_lang.ffi Require Import jrnl_ffi.
+From Perennial.goose_lang.ffi Require Import disk.
+From Goose.github_com.mit_pdos.goose_nfsd Require Import txn twophase.
+From Perennial.program_proof Require Import lockmap_proof.
+From Perennial.program_proof Require Import twophase.op_wrappers.
+From Perennial.program_proof Require Import addr.addr_proof buf.buf_proof txn.txn_proof.
+From Perennial.program_proof Require Import buftxn.sep_buftxn_proof.
+From Perennial.program_proof Require Import twophase.twophase_proof.
+From Perennial.goose_lang.lib.list Require Import list.
+From Perennial.goose_lang Require Import spec_assert.
+
+From Perennial.goose_lang Require Import ffi.disk_prelude.
+From Perennial.program_proof Require Import proof_prelude.
+
+Section proof.
+  Context `{!buftxnG Σ}.
+  Context `{!heapG Σ}.
+  Existing Instances jrnl_spec_ext jrnl_spec_ffi_model jrnl_spec_ext_semantics jrnl_spec_ffi_interp
+           jrnl_spec_interp_adequacy.
+  Context `{!refinement_heapG Σ}.
+
+  Implicit Types (N: namespace).
+
+  Definition is_twophase_system N γ :=
+    is_txn_system N γ.
+
+  Definition val_of_obj (o : obj) := val_of_list ((λ u, LitV (LitByte u)) <$> o).
+
+  Definition is_twophase_pre N l γ γ' dinit objs_dom : iProp Σ :=
+    ∃ (txnl locksl : loc) ghs,
+      let objs_dom_blknos := get_addr_set_blknos objs_dom in
+      "Histwophase_txnl" ∷ readonly (l ↦[TwoPhasePre.S :: "txn"] #txnl) ∗
+      "Histwophase_locksl" ∷ readonly (l ↦[TwoPhasePre.S :: "locks"] #locksl) ∗
+      "#Histxn_system" ∷ is_txn_system N γ ∗
+      "#Histxn" ∷ is_txn txnl γ.(buftxn_txn_names) dinit ∗
+      "#HlockMap" ∷ is_lockMap locksl ghs objs_dom_blknos (twophase_linv γ objs_dom) ∗
+      "#Htxn_cinv" ∷ txn_cinv N γ γ'.
+
+  Definition is_twophase_started N l γ γ' dinit objs_dom e1 e2 : iProp Σ :=
+    ∃ (txnl locksl : loc) ghs σj1 σj2,
+    let objs_dom_blknos := get_addr_set_blknos objs_dom in
+    "Htwophase.txn" ∷ readonly (l ↦[TwoPhase.S :: "txn"] #txnl) ∗
+    "Htwophase.locks" ∷ readonly (l ↦[TwoPhase.S :: "locks"] #locksl) ∗
+    "%Halways_steps" ∷ ⌜ always_steps e1 σj1 e2 σj2 ⌝ ∗
+    "#Histxn_system" ∷ is_txn_system N γ ∗
+    "#Histxn" ∷ is_txn txnl γ.(buftxn_txn_names) dinit ∗
+    "#HlockMap" ∷ is_lockMap locksl ghs objs_dom_blknos (twophase_linv γ objs_dom) ∗
+    "#Htxn_cinv" ∷ txn_cinv N γ γ' ∗
+    (* TODO: this should be at least all the na_crash_invs in σj1 and the ephemeral values
+       for σj2 *)
+    "Hlock_resources" ∷ True.
+
+  Definition is_twophase_committed N l γ γ' dinit objs_dom : iProp Σ :=
+    ∃ (txnl locksl : loc) ghs (σj : gmap addr obj),
+    let objs_dom_blknos := get_addr_set_blknos objs_dom in
+    "Htwophase.txn" ∷ readonly (l ↦[TwoPhase.S :: "txn"] #txnl) ∗
+    "Htwophase.locks" ∷ readonly (l ↦[TwoPhase.S :: "locks"] #locksl) ∗
+    "#Histxn_system" ∷ is_txn_system N γ ∗
+    "#Histxn" ∷ is_txn txnl γ.(buftxn_txn_names) dinit ∗
+    "#HlockMap" ∷ is_lockMap locksl ghs objs_dom_blknos (twophase_linv γ objs_dom) ∗
+    "#Htxn_cinv" ∷ txn_cinv N γ γ' ∗
+    (* TODO: this should be at least all the na_crash_invs in σj1 and the ephemeral values
+       for σj2 *)
+    "Hlock_resources" ∷ True.
+
+  Theorem wpc_Init' N (d: loc) γ dinit logm objs_dom k :
+    {{{ is_txn_durable γ dinit logm }}}
+      TwoPhase__Init' #d @ k; ⊤
+    {{{ γ' (l: loc), RET #l; is_twophase_pre N l γ γ' dinit objs_dom}}}
+    {{{ ∃ γ' logm', ⌜ γ'.(buftxn_txn_names).(txn_kinds) = γ.(buftxn_txn_names).(txn_kinds) ⌝ ∗
+        is_txn_durable γ' dinit logm' ∗
+       (⌜ γ' = γ ⌝ ∨ txn_cinv N γ γ') }}}.
+  Proof. Admitted.
+
+  Theorem wp_TwoPhase__Begin' N l γ γ' dinit objs_dom e1 a sz :
+    {{{ is_twophase_pre N l γ γ' dinit objs_dom}}}
+      TwoPhase__Begin' #l (addr2val a) #sz
+    {{{ tph, RET #tph;
+        is_twophase_started N tph γ γ' dinit objs_dom
+                            e1 e1 }}}.
+  Proof. Admitted.
+
+  Theorem wp_TwoPhase__CommitNoRelease' N l γ γ' dinit objs_dom  e1 e2 (j : nat) :
+    {{{ is_twophase_started N l γ γ' dinit objs_dom e1 e2 ∗
+        j ⤇ e1 }}}
+      TwoPhase__CommitNoRelease #l
+    {{{ (ok:bool), RET #ok;
+        if ok then
+          is_twophase_committed N l γ γ' dinit objs_dom ∗
+          j ⤇ e2
+        else
+          is_twophase_started N l γ γ' dinit objs_dom
+                              e1 e2 ∗
+          j ⤇ e1
+    }}}.
+  Proof. Admitted.
+
+  Theorem wp_TwoPhase__Release' N l γ γ' dinit objs_dom :
+    {{{ is_twophase_committed N l γ γ' dinit objs_dom }}}
+      TwoPhase__Release #l
+    {{{ RET #(); True }}}.
+  Proof. Admitted.
+
+  (* Among other things, this and the next spec are missing an assumption that
+     the kind/size is correct, so they cannot be proven as is. *)
+  Theorem wp_TwoPhase__ReadBuf' N l γ γ' dinit objs_dom K {HCTX: LanguageCtx K} e1 a sz :
+    {{{ is_twophase_started N l γ γ' dinit objs_dom
+                            e1
+                            (K (ExternalOp (ext := @spec_ext_op_field jrnl_spec_ext)
+                                           ReadBufOp (PairV (addr2val' a) #sz))) }}}
+      TwoPhase__ReadBuf' #l (addr2val a) #sz
+    {{{ v, RET (val_of_obj v);
+        is_twophase_started N l γ γ' dinit objs_dom
+                            e1 (K (val_of_obj' v)) }}}.
+  Proof. Admitted.
+
+  Theorem wp_TwoPhase__OverWrite' N l γ γ' dinit objs_dom K {HCTX: LanguageCtx K} e1 a ov :
+    {{{ is_twophase_started N l γ γ' dinit objs_dom
+                            e1
+                            (K (ExternalOp (ext := @spec_ext_op_field jrnl_spec_ext)
+                                           OverWriteOp (addr2val' a, val_of_obj' ov))) }}}
+      TwoPhase__OverWrite' #l (addr2val a) (val_of_obj ov)
+    {{{  RET #();
+        is_twophase_started N l γ γ' dinit objs_dom
+                            e1 (K #()) }}}.
+  Proof. Admitted.
+
+End proof.
